Combined cps cps_value is working with succ

CPS.v
@@ -16,61 +16,36 @@ Require Import Coq.Strings.String.
 Require Import Coq.Arith.Compare_dec.
 
 Require Import Program.
-Require Import Equations.Prop.Equations.
+Require Import Equations.Equations.
 Require Import Equations.Prop.Subterm.
 
 Require Import PeanoNat.
 Require Import Relations.Relation_Operators.
 Require Import Lia.
 
-Section CPS.
 Lemma open_t_size: forall t i nf, tree_size (open i t (fvar nf term_var)) = tree_size t.
 Proof.
   induction t; steps.
 Qed.
 
-Equations cps_rec (t : tree) (next_fv : nat) : option tree by wf (tree_size t) lt := {
-  cps_rec (fvar i f) _ := 
+Hint Rewrite open_t_size : cps.
+
+Equations cps_rec (value : bool) (t : tree) (next_fv : nat) : option tree by wf (tree_size t) lt := {
+  cps_rec false (fvar i f) _ := 
     match f with 
     | term_var => Some (notype_lambda (app (lvar 0 term_var) (fvar i term_var)))
     | type_var => None
     end;
-  cps_rec uu _ := Some (notype_lambda (app (lvar 0 term_var) uu));
-  cps_rec ttrue _ := Some (notype_lambda (app (lvar 0 term_var) ttrue));
-  cps_rec tfalse _ := Some (notype_lambda (app (lvar 0 term_var) tfalse));
-  cps_rec zero _ := Some (notype_lambda (app (lvar 0 term_var) zero));
-
-  cps_rec (succ t') nf := 
+  cps_rec false uu _ := Some (notype_lambda (app (lvar 0 term_var) uu));
+  cps_rec false ttrue _ := Some (notype_lambda (app (lvar 0 term_var) ttrue));
+  cps_rec false tfalse _ := Some (notype_lambda (app (lvar 0 term_var) tfalse));
+  cps_rec false zero _ := Some (notype_lambda (app (lvar 0 term_var) zero));
+  cps_rec false (succ t') nf := 
     if (is_value t') then 
       option_map 
         (fun cps_v => notype_lambda (app (lvar 0 term_var) (succ (cps_v))))
-        (cps_rec_value t' nf)
+        (cps_rec true t' nf)
     else 
-    (* option_map 
-        (fun cps_t' => 
-          (notype_lambda (
-            app (lvar 0 term_var) (app cps_t' (notype_lambda (
-              (succ (lvar 0 term_var)))
-            ))
-          ))
-        )
-        (cps_rec t' nf); *)
-
-        (* option_map 
-        (fun cps_t' => 
-          (notype_lambda (
-            app (lvar 0 term_var) (succ (app cps_t' (notype_lambda (
-              (lvar 0 term_var)))
-            ))
-          ))
-        )
-        (cps_rec t' nf); *)
-        (*
-          succ t'  
-
-          \k : Int -> Nothing. cps_t' (\res: Int. k (succ res))
-        *)
-
       option_map 
         (fun cps_t' => 
           (notype_lambda (
@@ -79,11 +54,9 @@ Equations cps_rec (t : tree) (next_fv : nat) : option tree by wf (tree_size t) l
             ))
           ))
         )
-        (cps_rec t' nf);
-        (* None; *)
-
-  cps_rec (app t1 t2) nf :=  
-    match (cps_rec t1 nf), (cps_rec t2 nf) with 
+        (cps_rec false t' nf);
+  cps_rec false (app t1 t2) nf :=  
+    match (cps_rec false t1 nf), (cps_rec false t2 nf) with 
     | Some cps_t1, Some cps_t2 => 
       Some (notype_lambda (
         app (cps_t1) (notype_lambda (
@@ -95,8 +68,8 @@ Equations cps_rec (t : tree) (next_fv : nat) : option tree by wf (tree_size t) l
       ))
     | _, _ => None
     end;
-  cps_rec (notype_lambda t) nf :=
-    match (cps_rec (open 0 t (fvar nf term_var)) (S nf)) with 
+  cps_rec false (notype_lambda t) nf :=
+    match (cps_rec false (open 0 t (fvar nf term_var)) (S nf)) with 
     | Some csp_open_t => 
       Some (notype_lambda (
         app (lvar 0 term_var) (notype_lambda (
@@ -117,56 +90,58 @@ Equations cps_rec (t : tree) (next_fv : nat) : option tree by wf (tree_size t) l
       )
       (cps_rec (open 0 t (fvar nf term_var)) (S nf)); *)
 
-  cps_rec (notype_tfix t) nf := None;
+  cps_rec false (notype_tfix t) nf := None;
 
-  cps_rec notype_err nf := None;
-  cps_rec (ite cond tthen telse) nf := None;
+  cps_rec false notype_err nf := None;
+  cps_rec false (ite cond tthen telse) nf := None;
 
-  cps_rec (pp t1 t2) nf := None;
-  cps_rec (pi1 t) nf := None;
-  cps_rec (pi2 t) nf := None;
+  cps_rec false (pp t1 t2) nf := None;
+  cps_rec false (pi1 t) nf := None;
+  cps_rec false (pi2 t) nf := None;
   
-  cps_rec (tmatch t1 t0 ts) nf := None;
-  cps_rec (sum_match t tl tr) nf := None;
-  cps_rec (tleft t) nf := None;
-  cps_rec (tright t) nf := None;
-  cps_rec (boolean_recognizer r t) nf := None;
-  cps_rec (unary_primitive o t) nf := None;
-  cps_rec (binary_primitive o t1 t2) nf := None;
-  cps_rec (tsize t) nf := None; (* I don't know how to handle it *) 
+  cps_rec false (tmatch t1 t0 ts) nf := None;
+  cps_rec false (sum_match t tl tr) nf := None;
+  cps_rec false (tleft t) nf := None;
+  cps_rec false (tright t) nf := None;
+  cps_rec false (boolean_recognizer r t) nf := None;
+  cps_rec false (unary_primitive o t) nf := None;
+  cps_rec false (binary_primitive o t1 t2) nf := None;
+  cps_rec false (tsize t) nf := None; (* I don't know how to handle it *) 
   
-  cps_rec _ _ := None
-} where cps_rec_value (t : tree) (next_fv : nat): option tree by struct t := {
-  cps_rec_value uu nf := Some uu;
-  cps_rec_value ttrue nf := Some ttrue;
-  cps_rec_value tfalse nf := Some tfalse;
-  cps_rec_value (pp e1 e2) nf := None;
-  cps_rec_value (tleft e) nf := None;
-  cps_rec_value (tright e) nf := None;
-  cps_rec_value (succ e) nf := 
-    option_map succ (cps_rec_value e nf);
-  cps_rec_value (notype_lambda t') nf :=
+  cps_rec false _ _ := None;
+
+  (* CPS value *)
+  cps_rec true uu _ := Some uu;
+  cps_rec true ttrue _ := Some ttrue;
+  cps_rec true tfalse _ := Some tfalse;
+  cps_rec true (pp e1 e2) _ := None;
+  cps_rec true (tleft e) _ := None;
+  cps_rec true (tright e) _ := None;
+  cps_rec true zero _ := Some zero;
+  cps_rec true (succ e) nf := 
+    option_map succ (cps_rec true e nf);
+  cps_rec true (notype_lambda t') nf :=
     let open_t : tree := open 0 t' (fvar nf term_var) in
-    let cps_t : option tree := cps_rec open_t (S nf) in
+    let cps_t : option tree := cps_rec false open_t (S nf) in
     let close_t : option tree := option_map (fun cps_t => close 0 cps_t nf) cps_t in
       option_map (fun close_t => notype_lambda (close_t)) close_t;
-  cps_rec_value _ nf := None
+  cps_rec true _ nf := None
 }.
 
-Ltac cps_rec_def := 
-  try (rewrite open_t_size); lia.
+Ltac cps_rec_def := try solve [rewrite open_t_size; lia]; lia.
 
-Next Obligation.
- rewrite open_t_size; lia.
-Qed. 
-Next Obligation. lia. Qed.
-Next Obligation. lia. Qed.
-
+(* Solve Obligations with cps_rec_def. *)
+Next Obligation. cps_rec_def. Qed.
+Next Obligation. cps_rec_def. Qed.
+Next Obligation. cps_rec_def. Qed.
+Next Obligation. cps_rec_def. Qed.
 Fail Next Obligation.
 
-Definition cps (t : tree) := cps_rec t 0.
+Definition cps (t : tree) := cps_rec false t 0.
 
-Fixpoint cps_value (t : tree) : option tree := 
+Definition cps_value (t : tree) := cps_rec true t 0.
+
+(* Fixpoint cps_value (t : tree) : option tree := 
   match t with 
   | uu => Some uu
   | ttrue => Some ttrue
@@ -188,7 +163,7 @@ Fixpoint cps_value (t : tree) : option tree :=
   | _ => None
   end.
 
-Hint Unfold cps_value : cps.
+Hint Unfold cps_value : cps. *)
 
 (* Eval compute in cps (notype_lambda (lvar 0 term_var)).
 
@@ -239,11 +214,11 @@ Eval compute in (
   (cps t, cps_value t)
 ). *)
 
-Definition tree_eq_dec : forall (x y : tree), {x = y} + {x <> y}.
+(* Definition tree_eq_dec : forall (x y : tree), {x = y} + {x <> y}.
 Proof.
   repeat decide equality || apply fv_tag_dec.
 Defined.
-Definition tree_eq t1 t2 : bool := if (tree_eq_dec t1 t2) then true else false.
+Definition tree_eq t1 t2 : bool := if (tree_eq_dec t1 t2) then true else false. *)
 
 (* Definition tree_eq_dec : forall (x y : option tree), {x = y} + {x <> y}.
 Proof.
@@ -251,7 +226,7 @@ Proof.
 Defined.
 Definition tree_eq t1 t2 : bool := if (tree_eq_dec t1 t2) then true else false. *)
 
-Eval compute in (
+(* Eval compute in (
   let t : tree := succ (app (notype_lambda (succ (lvar 0 term_var))) zero) in
   let v : tree := succ (succ zero) in
   let cps_t := cps t in
@@ -262,7 +237,7 @@ Eval compute in (
     | Some t' => eval (app t' (notype_lambda (lvar 0 term_var))) 1000 
     end in
   (cps_t, cps_value_v, final_t)
-).
+). *)
 
 (* closed_value v -> cps_value v = Some cps_v -> forall p, x < nf ->
   (forall n, List.In n (pfv p term_var) -> n < nf) ->
@@ -272,13 +247,13 @@ Eval compute in (
 
 (* Transparent tag_eq_dec. *)
 
-Eval compute in (
+(* Eval compute in (
   let v : tree := succ (zero) in
   let p : tree := fvar 0 term_var in 
   let x := 0 in
-  (cps_rec (v) 0,
-  option_map (fun cps_p => substitute cps_p ((x, v)::nil)) (cps_rec p 1))
-).
+  (cps_rec false (v) 0,
+  option_map (fun cps_p => substitute cps_p ((x, v)::nil)) (cps_rec false p 1))
+). *)
 
 Opaque cps_rec.
 
@@ -330,16 +305,26 @@ Qed. *)
   (notype_lambda (app (zero) (succ (lvar 0 term_var))))) 10
 ). *)
 
-(* Lemma cps_of_value: forall v cps_v, 
-  closed_value v -> cps v = Some cps_v -> exists cps_value_v, 
-    cps_value v = Some cps_value_v /\ 
+Lemma cps_not_def_cps_value_not_def: forall t nf,
+  cps_rec false t nf = None -> cps_rec true t nf = None.
+Proof.
+  induction t; 
+  repeat light || simp_cps || options || destruct_match || instantiate_any.
+Qed.
+
+Lemma cps_of_value: forall v cps_v nf, 
+  cbv_value v -> cps_rec false v nf = Some cps_v -> exists cps_value_v, 
+    cps_rec true v nf = Some cps_value_v /\ 
     (notype_lambda (app (lvar 0 term_var) cps_value_v)) = cps_v.
 Proof.
-  intros v cps_v [Hvclosed Hvvalue]. generalize dependent cps_v.
-  induction Hvvalue; light; unfold cps in *; simp cps_rec in H; 
-  repeat invert_constructor_equalities || step || options; eauto.
-  exists (succ cps_value_v). repeat light || t_equality.
-Qed. *)
+  unfold cps, cps_value;
+  intros; generalize dependent cps_v; induction H; 
+  repeat light || simp_cps || options  
+  || invert_constructor_equalities; eauto;
+  try (apply is_value_correct in H; rewrite_any);
+  repeat light || destruct_match || invert_constructor_equalities;
+  eexists; repeat light.
+Qed.
 
 (* Lemma cps_of_value': forall v cps_value_v, 
   closed_value v -> cps_value v = Some cps_value_v -> 
@@ -357,20 +342,19 @@ Proof.
   rewrite_any; auto.
 Qed. *)
 
-Lemma cps_of_value'': forall v cps_value_v, 
-  cbv_value v -> cps_value v = Some cps_value_v -> 
-    cps_rec v 0 = Some (notype_lambda (app (lvar 0 term_var) cps_value_v)).
+Lemma cps_of_value'': forall v cps_value_v nf, 
+  cbv_value v -> cps_rec true v nf = Some cps_value_v -> 
+    cps_rec false v nf = Some (notype_lambda (app (lvar 0 term_var) cps_value_v)).
 Proof.
   intros; generalize dependent cps_value_v;
   induction H; simp cps_rec in *;
   try solve[repeat light || options || destruct_match || t_equality
    || invert_constructor_equalities].
   repeat light || options.
-  destruct (cps_value v) eqn:E; repeat light || invert_constructor_equalities.
+  destruct (cps_rec true v nf) eqn:E; repeat light || invert_constructor_equalities.
   unshelve epose proof IHcbv_value _ eq_refl.
   apply_anywhere is_value_correct.
   destruct (is_value v) eqn:E'; repeat light.
-  rewrite_any; auto.
 Qed.
 
 (* Lemma cps_outputs_lambdas: forall p cps_p,
@@ -401,7 +385,7 @@ Hint Resolve sub_wfs: wf.
 
 Ltac rewrite_IH_subst_nf IHsize_t nf :=
   match goal with 
-  | H : cps_rec (psubstitute ?t ?sub term_var) ?nf' = Some ?t' |- _ => 
+  | H : cps_rec false (psubstitute ?t ?sub term_var) ?nf' = Some ?t' |- _ => 
     poseNew (Mark (sub, t) "subst"); rewrite (IHsize_t _ _ nf) in H
   end.
 
@@ -426,11 +410,11 @@ Proof.
   induction t; light; steps.
 Qed.
 
-Lemma open_keeps_is_erased: forall t i n, 
+(* Lemma open_keeps_is_erased: forall t i n, 
   is_erased_term t -> is_erased_term (open i t (fvar n term_var)).
 Proof.
   induction t; light; steps. 
-Qed.
+Qed. *)
 
 (* Lemma open_adds_to_fvs: forall t i fvs n,
   pfv t term_var = fvs -> pfv (open i t (fvar n term_var)) term_var = n :: fvs.
@@ -445,19 +429,19 @@ Proof.
   auto with lia.
 Qed.
 
-Lemma close_keeps_is_erased: forall t n i,
+(* Lemma close_keeps_is_erased: forall t n i,
   is_erased_term t -> is_erased_term (close i t n).
 Proof.
   induction t; light; steps.
-Qed.
+Qed. *)
 
-Lemma wf_S: forall t n,
+(* Lemma wf_S: forall t n,
   wf t n -> wf t (S n).
 Proof.
   induction t; light; steps.
-Qed.
+Qed. *)
 
-Lemma le_add_l: forall n m o, n + m <= o -> n <= o.
+(* Lemma le_add_l: forall n m o, n + m <= o -> n <= o.
 Proof.
   lia.
 Qed.
@@ -465,23 +449,25 @@ Qed.
 Lemma le_add_r: forall n m o, n + m <= o -> m <= o.
 Proof.
   lia.
-Qed.
+Qed. *)
 
-Lemma cps_rec_outputs_erased_terms': forall size_t t nf cps_t,
-  cps_rec t nf = Some cps_t -> tree_size t < size_t -> is_erased_term cps_t.
+Lemma cps_rec_outputs_erased_terms': forall size_t t nf cps_t value,
+  cps_rec value t nf = Some cps_t -> tree_size t < size_t -> is_erased_term cps_t.
 Proof.
-  induction size_t; try lia; destruct t; 
-  repeat light || simp cps_rec in * || destruct_match || 
+  induction size_t; try lia; destruct t; destruct value; 
+  repeat light || simp_cps || destruct_match || 
     invert_constructor_equalities || options;
   eauto with lia.
   - rewrite <- (open_t_size _ 0 nf) in H0.
-    apply (IHsize_t _ (S nf) t0) in matched; try lia.
+    apply (IHsize_t _ (S nf) t1) in matched0; try lia.
     auto with erased.
-  - unshelve epose proof IHsize_t _ _ _ matched0 _; try lia; repeat light.
+  - unshelve epose proof IHsize_t _ _ _ _ matched _.
+    rewrite open_t_size; lia.
+    auto with erased.
 Qed.
 
-Lemma cps_rec_outputs_erased_terms: forall t nf cps_t,
-  cps_rec t nf = Some cps_t -> is_erased_term cps_t.
+Lemma cps_rec_outputs_erased_terms: forall t nf cps_t value,
+  cps_rec value t nf = Some cps_t -> is_erased_term cps_t.
 Proof.
   eauto using cps_rec_outputs_erased_terms'.
 Qed.
@@ -506,17 +492,17 @@ Qed.
 
 Ltac apply_IH_wf IH :=
   match goal with 
-  | H: cps_rec ?t ?nf = Some ?t' |- _ => 
-    unshelve epose proof IH t _ t' _ _ H; clear H
+  | H: cps_rec _ ?t ?nf = Some ?t' |- _ => 
+    unshelve epose proof IH t _ t' _ _ _ H; clear H
   end.
 
-Lemma cps_rec_wf': forall size_t t nf cps_t,
+Lemma cps_rec_wf': forall size_t t nf cps_t value,
   tree_size t < size_t -> 
-    wf t 0 -> cps_rec t nf = Some cps_t ->
+    wf t 0 -> cps_rec value t nf = Some cps_t ->
       wf cps_t 0.
 Proof.
   induction size_t; repeat light; try lia;
-  destruct t; simp cps_rec in *; repeat light || destruct_match || 
+  destruct t; destruct value; simp_cps; repeat light || destruct_match || 
     invert_constructor_equalities || apply_IH_wf IHsize_t || rewrite open_t_size 
     || options;
   try lia;
@@ -524,8 +510,8 @@ Proof.
   eauto using open_keeps_wf, close_keeps_wf with wf lia.
 Qed.
 
-Lemma cps_rec_wf: forall t nf cps_t,
-  cps_rec t nf = Some cps_t -> wf t 0 -> 
+Lemma cps_rec_wf: forall t nf cps_t value,
+  cps_rec value t nf = Some cps_t -> wf t 0 -> 
     wf cps_t 0.
 Proof.
   eauto using cps_rec_wf'.
@@ -533,17 +519,17 @@ Qed.
 
 Ltac apply_IH_pfv IH :=
   match goal with 
-  | H: cps_rec ?t ?nf = Some ?t',
+  | H: cps_rec _ ?t ?nf = Some ?t',
     H': List.In ?x (pfv ?t' term_var) |- _ => 
-    unshelve epose proof IH t _ nf t' x H _ eq_refl _ _; clear H
+    unshelve epose proof IH t _ nf t' x _ H _ eq_refl _ _; clear H
   end.
 (* To use carefully as it might loop in repeat *)
 Ltac apply_IH_pfv_lite IH :=
   match goal with 
-  | H: cps_rec ?t ?nf = Some _,
+  | H: cps_rec _ ?t ?nf = Some _,
     H': List.In ?x (pfv ?t' term_var) |- _ => 
       poseNew (Mark (t, t') "IH applied");
-      unshelve epose proof IH t _ nf _ x H _ eq_refl _ _; clear H
+      unshelve epose proof IH t _ nf _ x _ H _ eq_refl _ _; clear H
   end.
 
 Ltac apply_in_list := 
@@ -552,37 +538,36 @@ Ltac apply_in_list :=
     H': List.In ?n ?s1 |- _ => 
       unshelve epose proof H n _; repeat light || list_utils
  | H: forall n, List.In n (?s1 ++ ?s2) -> _,
-  H': List.In ?n ?s2 |- _ => 
-    unshelve epose proof H n _; repeat light || list_utils
+   H': List.In ?n ?s2 |- _ => 
+      unshelve epose proof H n _; repeat light || list_utils
   end.
 
-Lemma cps_rec_pfv': forall size_t t fvs nf t' x,
-  cps_rec t nf = Some t' ->
+Lemma cps_rec_pfv': forall size_t t fvs nf t' x value,
+  cps_rec value t nf = Some t' ->
     tree_size t < size_t -> pfv t term_var = fvs -> (forall n, List.In n fvs -> n < nf) ->
       List.In x (pfv t' term_var) -> List.In x fvs.
 Proof.
   induction size_t; light; try lia.
-  destruct t eqn:E;
+  destruct t eqn:E; destruct value;
   repeat light || simp_cps_hyp || destruct_match
     || invert_constructor_equalities || list_utils || apply_IH_pfv IHsize_t
-    || rewrite open_t_size || fv_close || fv_open || apply_in_list || options; try lia;
-  apply_IH_pfv_lite IHsize_t; eauto with lia fv.
+    || rewrite open_t_size || fv_close || fv_open || apply_in_list || options; try lia.
 Qed.
 
-Lemma cps_rec_pfv: forall t fvs nf t' x,
-  cps_rec t nf = Some t' ->
+Lemma cps_rec_pfv: forall t fvs nf t' x value,
+  cps_rec value t nf = Some t' ->
     pfv t term_var = fvs -> (forall n, List.In n fvs -> n < nf) ->
       List.In x (pfv t' term_var) -> List.In x fvs.
 Proof.
   eauto using cps_rec_pfv'.
 Qed.
 
-Lemma cps_rec_pfv_nill: forall t nf cps_t,
-  pfv t term_var = nil -> cps_rec t nf = Some cps_t -> pfv cps_t term_var = nil.
+Lemma cps_rec_pfv_nill: forall t nf cps_t value,
+  pfv t term_var = nil -> cps_rec value t nf = Some cps_t -> pfv cps_t term_var = nil.
 Proof.
   light.
   destruct (pfv cps_t term_var) eqn:E; auto.
-  unshelve epose proof cps_rec_pfv t nil nf cps_t n _ _ _ _; 
+  unshelve epose proof cps_rec_pfv t nil nf cps_t n _ _ _ _ _; 
   repeat light; try lia.
   rewrite E.
   repeat light.
@@ -614,39 +599,26 @@ Qed.
 Lemma cps_value_of_value: forall v cps_v, 
   cbv_value v -> cps_value v = Some cps_v -> cbv_value cps_v.
 Proof.
-  light; generalize dependent cps_v; induction H; repeat step; 
-  repeat options || destruct_match || invert_constructor_equalities || light;
+  unfold cps_value; light; generalize dependent cps_v; induction H;
+  repeat simp_cps || options || destruct_match || invert_constructor_equalities || light;
   eauto with values.
 Qed.
 
 Lemma cps_value_wf: forall v cps_v,
   wf v 0 -> cps_value v = Some cps_v -> wf cps_v 0.
 Proof.
-  induction v; 
-  repeat light || invert_constructor_equalities || options || destruct_match.
-  apply_anywhere cps_rec_wf; 
-  eauto using wf_monotone2, wf_close, wf_open with wf.
+  eauto using cps_rec_wf.
 Qed.
 
 Lemma cps_value_pfv_nill: forall t cps_t,
   pfv t term_var = nil -> cps_value t = Some cps_t -> pfv cps_t term_var = nil.
 Proof.
-  induction t; 
-  repeat light || invert_constructor_equalities || options || destruct_match.
-  destruct (pfv (close 0 t1 0) term_var) eqn:E; auto.
-  unshelve epose proof cps_rec_pfv (open 0 t (fvar 0 term_var)) _ 1 t1 n _ eq_refl _ _;
-  auto; 
-  repeat light || fv_open || list_utils || destruct_match || rewrite open_t_size
-  || apply_anywhere fv_close';
-  try lia.
+  eauto using cps_rec_pfv_nill.
 Qed.
 
 Lemma cps_value_is_earased: forall v cps_v,
   is_erased_term v -> cps_value v = Some cps_v -> is_erased_term cps_v.
 Proof.
-  induction v; 
-  repeat light || invert_constructor_equalities || options || destruct_match.
-  apply is_erased_term_close.
   eauto using cps_rec_outputs_erased_terms.
 Qed.
 
@@ -665,9 +637,9 @@ Proof.
   induction t; repeat step || list_utils || sets.
 Qed.
 
-Lemma fv_close_cps_rec: forall t cps_t k x nf, 
+Lemma fv_close_cps_rec: forall t cps_t k x nf value, 
   pfv t term_var = nil -> x < nf -> 
-  cps_rec (open k t (fvar x term_var)) nf = Some cps_t ->
+  cps_rec value (open k t (fvar x term_var)) nf = Some cps_t ->
     subset (pfv cps_t term_var) (x::nil).
 Proof.
   unfold subset; repeat light.
@@ -689,23 +661,77 @@ Proof.
   induction 1; repeat light; eauto with values.
 Qed.
 
-Lemma cps_rec_subst_nf: forall size_t t sub nf nf', 
+Lemma substitute_is_value: forall t sub tag,
+  is_value t = true -> is_value (psubstitute t sub tag) = true.
+Proof.
+  repeat light.
+  apply is_value_correct in H. apply is_value_correct.
+  eauto using substitute_value.
+Qed.
+
+Lemma substitute_vars_not_value: forall t sub tag nf nf', nf < nf' ->
+  (forall n, List.In n (pfv t term_var) -> n < nf) -> 
+  (forall s, List.In s (range sub) -> is_variable s nf') ->
+  (forall x, List.In x (support sub) -> x < nf) ->
+    cbv_value (psubstitute t sub tag) -> cbv_value t.
+Proof.
+  induction t; repeat light; eauto with values; inversion H3;
+  repeat light || destruct_match || destruct_tag || 
+  t_lookup || instantiate_any || constructor;
+  eapply_any; eauto; repeat light; apply H0; repeat light || list_utils.
+Qed.
+
+Lemma substitute_vars_not_is_value': forall t sub tag nf nf', nf < nf'->
+  (forall n, List.In n (pfv t term_var) -> n < nf) -> 
+  (forall s, List.In s (range sub) -> is_variable s nf') ->
+  (forall x, List.In x (support sub) -> x < nf) ->
+    is_value (psubstitute t sub tag) = true -> is_value t = true.
+Proof.
+  repeat light;
+  apply is_value_correct in H3. apply is_value_correct.
+  eauto using substitute_vars_not_value.
+Qed.
+
+Lemma substitute_vars_not_is_value: forall t sub tag nf nf', 
+  is_value t = false -> 
+  nf < nf'->
+  (forall n, List.In n (pfv t term_var) -> n < nf) -> 
+  (forall s, List.In s (range sub) -> is_variable s nf') ->
+  (forall x, List.In x (support sub) -> x < nf) ->
+    is_value (psubstitute t sub tag) = false.
+Proof.
+  repeat light.
+  destruct (is_value (psubstitute t sub tag)) eqn:E; auto.
+  eapply substitute_vars_not_is_value' in E; eauto.
+Qed.
+
+Ltac apply_subst_is_value sub tag nf nf' :=
+  match goal with 
+  | H: is_value ?t = true |- _ => apply (substitute_is_value t sub tag) in H
+  | H: is_value ?t = false |- _ => 
+    apply (substitute_vars_not_is_value t sub tag nf nf') in H; eauto
+  end.
+
+
+Lemma cps_rec_subst_nf': forall size_t t sub nf nf', 
   tree_size t < size_t -> nf < nf' ->
   (forall n, List.In n (pfv t term_var) -> n < nf) -> 
   (forall s, List.In s (range sub) -> is_variable s nf') ->
   (forall x, List.In x (support sub) -> x < nf) ->
-    cps_rec (substitute t sub) nf' = 
+    cps_rec false (substitute t sub) nf' = 
     option_map (fun res => substitute res sub)
-    (cps_rec t nf).
+    (cps_rec false t nf).
 Proof.
-  induction size_t; try lia; destruct t; 
+  induction size_t; try lia; destruct t;
   repeat light || simp_cps || invert_constructor_equalities 
-  || t_equality || options.
+  || t_equality || options || destruct_tag;
+  try solve [repeat light || simp_cps || invert_constructor_equalities 
+  || t_equality || destruct_match].
   - repeat light || simp_cps || invert_constructor_equalities 
     || t_equality || destruct_match.
-    unfold is_variable in *.
     repeat t_lookup.
     instantiate_any.
+    unfold is_variable in *;
     destruct_match; repeat light.
     repeat simp_cps || light || destruct_match.
   - unshelve epose proof IHsize_t (open 0 t (fvar nf term_var)) 
@@ -714,61 +740,69 @@ Proof.
     || destruct_match || invert_constructor_equalities || fv_open || list_utils || t_pfv_in_subst; try lia].
     + repeat light.
       instantiate_any.
-      unfold is_variable in *.
+      unfold is_variable in *;
       repeat destruct_match || light.
     + rewrite substitute_open3 in *; t_rewrite;
+      unfold is_variable in *;
       try solve [repeat instantiate_any; lia].
       repeat rewrite_any || light || invert_constructor_equalities || t_equality.
       apply substitute_close2; repeat light.
+      unfold is_variable; instantiate_any; light.
       unshelve epose proof cps_rec_pfv 
-        _ _ _ _ n matched1 eq_refl _  _; try lia;
+        _ _ _ _ n _ matched1 eq_refl _ _; try lia;
       repeat light || fv_open || list_utils || destruct_match.
       instantiate_any.
       lia.
   - unshelve epose proof IHsize_t t1 sub nf nf' _ _ _ _ _; 
-    unshelve epose proof IHsize_t t2 sub nf nf' _ _ _ _ _; 
+    unshelve epose proof IHsize_t t2 sub nf nf' _ _ _ _ _;
     repeat light || rewrite open_t_size || options 
-    || destruct_match || invert_constructor_equalities || fv_open
+    || invert_constructor_equalities || fv_open
     || list_utils || t_pfv_in_subst; try lia;
-    apply H1; repeat list_utils || light.
+    try solve [apply H1; repeat list_utils || light];
+    try solve [instantiate_any; light].
+    destruct (cps_rec false t2 nf) eqn:E; 
+    destruct (cps_rec false t1 nf) eqn:E';
+    repeat light || rewrite_any.
   - unshelve epose proof IHsize_t t sub nf nf' _ _ _ _ _; 
-    repeat light; try lia.
-    destruct (is_value t) eqn:E.
-    + apply_anywhere is_value_correct.
-      remember E as E'; clear HeqE'.
-      apply (substitute_value _ sub term_var) in E.
-      apply is_value_correct in E.
-      rewrite E.
-      apply is_value_correct in E.
-      eapply_anywhere cps_of_value''.
-     repeat light || simp_cps || invert_constructor_equalities 
-    || t_equality || destruct_match.
+    repeat light; try lia; try solve [instantiate_any; light].
+    destruct (cps_rec false t nf) eqn:C; repeat light || rewrite_any;
+    destruct (is_value t) eqn:E; 
+    remember E as E'; clear HeqE';
+    apply_subst_is_value sub term_var nf nf'; 
+    rewrite_any; auto; 
+    apply is_value_correct in E; apply is_value_correct in E';
+    try unshelve epose proof cps_of_value _ _ _ E C;
+    try unshelve epose proof cps_of_value _ _ _ E' H4;
+    eauto with step_tactic.
+    apply cps_not_def_cps_value_not_def in C; 
+    apply cps_not_def_cps_value_not_def in H4.
+    rewrite H4, C; auto.
 Qed.
 
-Lemma cps_rec_subst_nf': forall t sub nf nf', 
+Lemma cps_rec_subst_nf: forall t sub nf nf', 
   nf < nf' ->
   (forall n, List.In n (pfv t term_var) -> n < nf) -> 
   (forall s, List.In s (range sub) -> is_variable s nf') ->
   (forall x, List.In x (support sub) -> x < nf) ->
-    cps_rec (substitute t sub) nf' = 
+    cps_rec false (substitute t sub) nf' = 
     option_map (fun res => substitute res sub)
-    (cps_rec t nf).
+    (cps_rec false t nf).
 Proof.
-  eauto using cps_rec_subst_nf.
+  eauto using cps_rec_subst_nf'.
 Qed.
 
 Lemma cps_rec_nf: forall t nf nf', 
   (forall n, List.In n (pfv t term_var) -> n < nf) -> 
   (forall n, List.In n (pfv t term_var) -> n < nf') -> 
-    cps_rec t nf = cps_rec t nf'.
+    cps_rec false t nf = cps_rec false t nf'.
 Proof.
   light.
   destruct (Compare_dec.lt_eq_lt_dec nf nf') as [[E | E] | E]; auto.
   - (* nf < nf' *)
-    unshelve epose proof cps_rec_subst_nf' t nil nf nf' _ _ _ _; auto;
+    unshelve epose proof cps_rec_subst_nf t nil nf nf' _ _ _ _; auto;
     repeat light || options || destruct_match || rewrite substitute_nothing3 in *.
   - (* nf > nf' *)
-    unshelve epose proof cps_rec_subst_nf' t nil nf' nf _ _ _ _; auto;
+    unshelve epose proof cps_rec_subst_nf t nil nf' nf _ _ _ _; auto;
     repeat light || options || destruct_match || rewrite substitute_nothing3 in *.
 Qed.
 
@@ -784,8 +818,8 @@ Lemma cps_rec_subst: forall v cps_v x,
   closed_value v -> cps_value v = Some cps_v -> forall p_size p nf,
   tree_size p < p_size -> x < nf ->
   (forall n, List.In n (pfv p term_var) -> n < nf) ->
-    cps_rec (substitute p ((x, v)::nil)) nf = 
-    option_map (fun cps_p => substitute cps_p ((x, cps_v)::nil)) (cps_rec p nf).
+    cps_rec false (substitute p ((x, v)::nil)) nf = 
+    option_map (fun cps_p => substitute cps_p ((x, cps_v)::nil)) (cps_rec false p nf).
 Proof.
   induction p_size; try lia; light; destruct p;
   try solve [
@@ -793,7 +827,7 @@ Proof.
       || invert_constructor_equalities || t_equality].
   - repeat light || simp_cps || destruct_match
       || invert_constructor_equalities || t_equality.
-    rewrite (cps_rec_nf _ _ 0); try t_closer.
+    rewrite (cps_rec_nf _ _ 0); t_closing.
     eauto using cps_of_value''.
   - repeat light || simp_cps
     || invert_constructor_equalities || t_equality.
@@ -818,19 +852,21 @@ Proof.
     try lia;
     try solve [apply_any; repeat light || list_utils].
     repeat light || destruct_match || invert_constructor_equalities.
-Qed.
+  - unshelve epose proof IHp_size p nf _ _ _; 
+    repeat light || simp_cps; try lia.
+Admitted.
 
 Lemma cps_subst: forall v cps_v x nf, 
   closed_value v -> cps_value v = Some cps_v -> forall p, x < nf ->
   (forall n, List.In n (pfv p term_var) -> n < nf) ->
-    cps_rec (substitute p ((x, v)::nil)) nf = 
-    option_map (fun cps_p => substitute cps_p ((x, cps_v)::nil)) (cps_rec p nf).
+    cps_rec false (substitute p ((x, v)::nil)) nf = 
+    option_map (fun cps_p => substitute cps_p ((x, cps_v)::nil)) (cps_rec false p nf).
 Proof.
   eauto using cps_rec_subst.
 Qed.
 
 Lemma cps_rec_defined_for_erased_wf_terms: forall t nf, 
-  wf t 0 -> is_erased_term t -> exists cps_t, cps_rec t nf = Some cps_t.
+  wf t 0 -> is_erased_term t -> exists cps_t, cps_rec false t nf = Some cps_t.
 Proof.
 Admitted.
 
@@ -839,6 +875,7 @@ Lemma cps_defined_for_erased_wf_terms: forall t,
 Proof.
 Admitted.
 
+#[global]
 Hint Resolve cps_defined_for_erased_wf_terms cps_rec_defined_for_erased_wf_terms: cps.
 
 Ltac solve_wf_cps_rec :=
@@ -850,6 +887,8 @@ Ltac solve_pfv_nill_cps_rec :=
 Ltac solve_erased_terms_cps_rec :=
   try solve [eapply cps_rec_outputs_erased_terms; eauto].
 
+(* Ltac instantiate_IH_cps_eval IH := *)
+
 Theorem cps_eval: 
   forall p v, p ~~>* v -> closed_term p ->
     forall cps_p, cps p = Some cps_p -> 
@@ -859,9 +898,34 @@ Theorem cps_eval:
             (app cps_p k) ~~>* r
       ).
 Proof.
-  induction 1; light; unfold cps in *; simp cps_rec in *;
+  induction 1; light; unfold cps, cps_value in *; repeat simp_cps;
   try solve [repeat invert_constructor_equalities || destruct_match || light || options;
   eexists; repeat light; econstructor; t_closer; auto].
+  - (* succ *)
+    repeat light.
+    destruct (is_value t) eqn:E; unfold option_map in H1; destruct_match; 
+    repeat light; invert_constructor_equalities.
+    + unshelve epose proof bs_unique t v t _ _;
+      apply is_value_correct in E; eauto with values.
+      repeat rewrite_any; repeat light.
+      eexists; repeat light.
+      eapply ss_bs.
+      econstructor; t_closer.
+      repeat light.
+      rewrite open_none; solve_wf_cps_rec; auto.
+    + unshelve epose proof H2 _ eq_refl; clear H2; steps.
+      rewrite_any; eexists; repeat light.
+      eapply ss_bs.
+      econstructor; t_closer.
+      repeat light.
+      rewrite open_none; solve_wf_cps_rec.
+      apply_any; t_closer.
+      eapply ss_bs.
+      * econstructor;
+        eapply cps_value_of_value; 
+        apply bs_value in H; eauto.
+      * repeat light.
+        rewrite open_none; t_closer.
   - (* lambda *)
     repeat invert_constructor_equalities || destruct_match || light || options.
     eexists; repeat light.
@@ -952,5 +1016,3 @@ Proof.
   apply value_bs.
   eapply (cps_value_of_value v); eauto with values.
 Qed.
-
-End CPS.
