BigStep.v
@@ -10,7 +10,9 @@ Inductive bcbv_step: tree -> tree -> Prop :=
   | BSttrue : ttrue ~~>* ttrue
   | BStfalse : tfalse ~~>* tfalse
   | BSzero : zero ~~>* zero
-
+  | BSsucc : forall t v,
+    t ~~>* v ->
+      succ t ~~>* succ v
   (* lambda *)
   | BSlambda : forall t, 
       notype_lambda t ~~>* notype_lambda t 
@@ -21,6 +23,7 @@ Inductive bcbv_step: tree -> tree -> Prop :=
         app t1 t2 ~~>* v
 where "t '~~>*' v" := (bcbv_step t v).
 
+#[global]
 Hint Constructors bcbv_step : bcbv_step.
 
 Lemma bs_closed_term: forall t1 t2, t1 ~~>* t2 -> closed_term t1 -> closed_term t2.
@@ -38,8 +41,18 @@ Proof.
   induction 1.
 Admitted.
 
+#[global]
 Hint Immediate bs_value value_bs : values.
 
+Lemma bs_unique: forall t v1 v2, 
+  t ~~>* v1 -> 
+  t ~~>* v2 ->
+    v1 = v2.
+Proof.
+  intros; generalize dependent v2;
+  induction H; inversion 1; 
+  repeat light || t_equality || instantiate_any || invert_constructor_equalities. 
+Qed.
 
 (* Equivalance small step*)
 
